Extracted list_numbers.v with seq, seqZ, sum_list and max_list

theories/list.v
@@ -401,12 +401,6 @@ used by [positives_flatten]. *)
 Definition positives_unflatten (p : positive) : option (list positive) :=
   positives_unflatten_go p [] 1.
 
-(** [seqZ m n] generates the sequence [m], [m + 1], ..., [m + n - 1]
-over integers, provided [0 ≤ n]. If [n < 0], then the range is empty. **)
-Definition seqZ (m len: Z) : list Z :=
-  (λ i: nat, Z.add i m) <$> (seq 0 (Z.to_nat len)).
-Arguments seqZ : simpl never.
-
 (** * Basic tactics on lists *)
 (** The tactic [discriminate_list] discharges a goal if it submseteq
 a list equality involving [(::)] and [(++)] of two lists that have a different
@@ -1036,14 +1030,6 @@ Proof.
   intros l1 l2 Hl.
   by rewrite <-(reverse_involutive l1), <-(reverse_involutive l2), Hl.
 Qed.
-Lemma sum_list_with_app (f : A → nat) l k :
-  sum_list_with f (l ++ k) = sum_list_with f l + sum_list_with f k.
-Proof. induction l; simpl; lia. Qed.
-Lemma sum_list_with_reverse (f : A → nat) l :
-  sum_list_with f (reverse l) = sum_list_with f l.
-Proof.
-  induction l; simpl; rewrite ?reverse_cons, ?sum_list_with_app; simpl; lia.
-Qed.
 
 (** ** Properties of the [last] function *)
 Lemma last_snoc x l : last (l ++ [x]) = Some x.
@@ -1371,14 +1357,6 @@ Proof. intros. by rewrite !list_lookup_total_alt, lookup_resize_old. Qed.
 (** ** Properties of the [reshape] function *)
 Lemma reshape_length szs l : length (reshape szs l) = length szs.
 Proof. revert l. by induction szs; intros; f_equal/=. Qed.
-Lemma join_reshape szs l :
-  sum_list szs = length l → mjoin (reshape szs l) = l.
-Proof.
-  revert l. induction szs as [|sz szs IH]; simpl; intros l Hl; [by destruct l|].
-  by rewrite IH, take_drop by (rewrite drop_length; lia).
-Qed.
-Lemma sum_list_replicate n m : sum_list (replicate m n) = m * n.
-Proof. induction m; simpl; auto. Qed.
 End general_properties.
 
 Section more_general_properties.
@@ -3615,128 +3593,6 @@ Section imap.
     x ∈ imap f l ↔ ∃ i y, x = f i y ∧ l !! i = Some y.
   Proof. naive_solver eauto using elem_of_lookup_imap_1, elem_of_lookup_imap_2. Qed.
 End imap.
-
-
-(** ** Properties of the [seq] function *)
-Section seq.
-  Implicit Types m n i j : nat.
-
-  Lemma fmap_add_seq j j' n : Nat.add j <$> seq j' n = seq (j + j') n.
-  Proof.
-    revert j'. induction n as [|n IH]; intros j'; csimpl; [reflexivity|].
-    by rewrite IH, Nat.add_succ_r.
-  Qed.
-  Lemma fmap_S_seq j n : S <$> seq j n = seq (S j) n.
-  Proof. apply (fmap_add_seq 1). Qed.
-  Lemma imap_seq {A} (l : list A) (g : nat → A) i :
-    imap (λ j _, g (i + j)) l = g <$> seq i (length l).
-  Proof.
-    revert i. induction l as [|x l IH]; [done|].
-    csimpl. intros n. rewrite <-IH, <-plus_n_O. f_equal.
-    apply imap_ext; simpl; auto with lia.
-  Qed.
-  Lemma imap_seq_0 {A} (l : list A) (g : nat → A) :
-    imap (λ j _, g j) l = g <$> seq 0 (length l).
-  Proof. rewrite (imap_ext _ (λ i o, g (0 + i))); [|done]. apply imap_seq. Qed.
-  Lemma lookup_seq_lt j n i : i < n → seq j n !! i = Some (j + i).
-  Proof.
-    revert j i. induction n as [|n IH]; intros j [|i] ?; simpl; auto with lia.
-    rewrite IH; auto with lia.
-  Qed.
-  Lemma lookup_total_seq_lt j n i : i < n → seq j n !!! i = j + i.
-  Proof. intros. by rewrite !list_lookup_total_alt, lookup_seq_lt. Qed.
-  Lemma lookup_seq_ge j n i : n ≤ i → seq j n !! i = None.
-  Proof. revert j i. induction n; intros j [|i] ?; simpl; auto with lia. Qed.
-  Lemma lookup_total_seq_ge j n i : n ≤ i → seq j n !!! i = inhabitant.
-  Proof. intros. by rewrite !list_lookup_total_alt, lookup_seq_ge. Qed.
-  Lemma lookup_seq j n i j' : seq j n !! i = Some j' ↔ j' = j + i ∧ i < n.
-  Proof.
-    destruct (le_lt_dec n i).
-    - rewrite lookup_seq_ge by done. naive_solver lia.
-    - rewrite lookup_seq_lt by done. naive_solver lia.
-  Qed.
-  Lemma NoDup_seq j n : NoDup (seq j n).
-  Proof. apply NoDup_ListNoDup, seq_NoDup. Qed.
-  Lemma seq_S_end_app j n : seq j (S n) = seq j n ++ [j + n].
-  Proof.
-    revert j. induction n as [|n IH]; intros j; simpl in *; f_equal; [done |].
-    by rewrite IH, Nat.add_succ_r.
-  Qed.
-
-  Lemma Forall_seq (P : nat → Prop) i n :
-    Forall P (seq i n) ↔ ∀ j, i ≤ j < i + n → P j.
-  Proof.
-    rewrite Forall_lookup. split.
-    - intros H j [??]. apply (H (j - i)), lookup_seq. lia.
-    - intros H j x [-> ?]%lookup_seq. auto with lia.
-  Qed.
-End seq.
-
-
-(** ** Properties of the [seqZ] function *)
-Section seqZ.
-  Implicit Types (m n : Z) (i j : nat).
-  Local Open Scope Z.
-
-  Lemma seqZ_nil m n : n ≤ 0 → seqZ m n = [].
-  Proof. by destruct n. Qed.
-  Lemma seqZ_cons m n : 0 < n → seqZ m n = m :: seqZ (Z.succ m) (Z.pred n).
-  Proof.
-    intros H. unfold seqZ. replace n with (Z.succ (Z.pred n)) at 1 by lia.
-    rewrite Z2Nat.inj_succ by lia. f_equal/=.
-    rewrite <-fmap_S_seq, <-list_fmap_compose.
-    apply map_ext; naive_solver lia.
-  Qed.
-  Lemma seqZ_length m n : length (seqZ m n) = Z.to_nat n.
-  Proof. unfold seqZ; by rewrite fmap_length, seq_length. Qed.
-  Lemma fmap_add_seqZ m m' n : Z.add m <$> seqZ m' n = seqZ (m + m') n.
-  Proof.
-    revert m'. induction n as [|n ? IH|] using (Z_succ_pred_induction 0); intros m'.
-    - by rewrite seqZ_nil.
-    - rewrite (seqZ_cons m') by lia. rewrite (seqZ_cons (m + m')) by lia.
-      f_equal/=. rewrite Z.pred_succ, IH; simpl. f_equal; lia.
-    - by rewrite !seqZ_nil by lia.
-  Qed.
-  Lemma lookup_seqZ_lt m n i : i < n → seqZ m n !! i = Some (m + i).
-  Proof.
-    revert m i. induction n as [|n ? IH|] using (Z_succ_pred_induction 0);
-      intros m i Hi; [lia| |lia].
-    rewrite seqZ_cons by lia. destruct i as [|i]; simpl.
-    - f_equal; lia.
-    - rewrite Z.pred_succ, IH by lia. f_equal; lia.
-  Qed.
-  Lemma lookup_total_seqZ_lt m n i : i < n → seqZ m n !!! i = m + i.
-  Proof. intros. by rewrite !list_lookup_total_alt, lookup_seqZ_lt. Qed.
-  Lemma lookup_seqZ_ge m n i : n ≤ i → seqZ m n !! i = None.
-  Proof.
-    revert m i.
-    induction n as [|n ? IH|] using (Z_succ_pred_induction 0); intros m i Hi; try lia.
-    - by rewrite seqZ_nil.
-    - rewrite seqZ_cons by lia.
-      destruct i as [|i]; simpl; [lia|]. by rewrite Z.pred_succ, IH by lia.
-    - by rewrite seqZ_nil by lia.
-  Qed.
-  Lemma lookup_total_seqZ_ge m n i : n ≤ i → seqZ m n !!! i = inhabitant.
-  Proof. intros. by rewrite !list_lookup_total_alt, lookup_seqZ_ge. Qed.
-  Lemma lookup_seqZ m n i m' : seqZ m n !! i = Some m' ↔ m' = m + i ∧ i < n.
-  Proof.
-    destruct (Z_le_gt_dec n i).
-    - rewrite lookup_seqZ_ge by lia. naive_solver lia.
-    - rewrite lookup_seqZ_lt by lia. naive_solver lia.
-  Qed.
-  Lemma NoDup_seqZ m n : NoDup (seqZ m n).
-  Proof. apply NoDup_fmap_2, NoDup_seq. intros ???; lia. Qed.
-
-  Lemma Forall_seqZ (P : Z → Prop) m n :
-    Forall P (seqZ m n) ↔ ∀ m', m ≤ m' < m + n → P m'.
-  Proof.
-    rewrite Forall_lookup. split.
-    - intros H j [??]. apply (H (Z.to_nat (j - m))), lookup_seqZ.
-      rewrite !Z2Nat.id by lia. lia.
-    - intros H j x [-> ?]%lookup_seqZ. auto with lia.
-  Qed.
-End seqZ.
-
 
 (** ** Properties of the [permutations] function *)
 Section permutations.
