theories/list_numbers.v
@@ -1,0 +1,173 @@
+(** This file collects general purpose definitions and theorems on
+lists of numbers that are not in the Coq standard library. *)
+From stdpp Require Export list.
+Set Default Proof Using "Type*".
+
+(** * Definitions *)
+(** [seqZ m n] generates the sequence [m], [m + 1], ..., [m + n - 1]
+over integers, provided [0 ≤ n]. If [n < 0], then the range is empty. **)
+Definition seqZ (m len: Z) : list Z :=
+  (λ i: nat, Z.add i m) <$> (seq 0 (Z.to_nat len)).
+Arguments seqZ : simpl never.
+
+Definition sum_list_with {A} (f : A → nat) : list A → nat :=
+  fix go l :=
+  match l with
+  | [] => 0
+  | x :: l => f x + go l
+  end.
+Notation sum_list := (sum_list_with id).
+
+Definition max_list_with {A} (f : A → nat) : list A → nat :=
+  fix go l :=
+  match l with
+  | [] => 0
+  | x :: l => f x `max` go l
+  end.
+Notation max_list := (max_list_with id).
+
+(** * Properties *)
+(** ** Properties of the [seq] function *)
+Section seq.
+  Implicit Types m n i j : nat.
+
+  Lemma fmap_add_seq j j' n : Nat.add j <$> seq j' n = seq (j + j') n.
+  Proof.
+    revert j'. induction n as [|n IH]; intros j'; csimpl; [reflexivity|].
+    by rewrite IH, Nat.add_succ_r.
+  Qed.
+  Lemma fmap_S_seq j n : S <$> seq j n = seq (S j) n.
+  Proof. apply (fmap_add_seq 1). Qed.
+  Lemma imap_seq {A} (l : list A) (g : nat → A) i :
+    imap (λ j _, g (i + j)) l = g <$> seq i (length l).
+  Proof.
+    revert i. induction l as [|x l IH]; [done|].
+    csimpl. intros n. rewrite <-IH, <-plus_n_O. f_equal.
+    apply imap_ext; simpl; auto with lia.
+  Qed.
+  Lemma imap_seq_0 {A} (l : list A) (g : nat → A) :
+    imap (λ j _, g j) l = g <$> seq 0 (length l).
+  Proof. rewrite (imap_ext _ (λ i o, g (0 + i))); [|done]. apply imap_seq. Qed.
+  Lemma lookup_seq_lt j n i : i < n → seq j n !! i = Some (j + i).
+  Proof.
+    revert j i. induction n as [|n IH]; intros j [|i] ?; simpl; auto with lia.
+    rewrite IH; auto with lia.
+  Qed.
+  Lemma lookup_total_seq_lt j n i : i < n → seq j n !!! i = j + i.
+  Proof. intros. by rewrite !list_lookup_total_alt, lookup_seq_lt. Qed.
+  Lemma lookup_seq_ge j n i : n ≤ i → seq j n !! i = None.
+  Proof. revert j i. induction n; intros j [|i] ?; simpl; auto with lia. Qed.
+  Lemma lookup_total_seq_ge j n i : n ≤ i → seq j n !!! i = inhabitant.
+  Proof. intros. by rewrite !list_lookup_total_alt, lookup_seq_ge. Qed.
+  Lemma lookup_seq j n i j' : seq j n !! i = Some j' ↔ j' = j + i ∧ i < n.
+  Proof.
+    destruct (le_lt_dec n i).
+    - rewrite lookup_seq_ge by done. naive_solver lia.
+    - rewrite lookup_seq_lt by done. naive_solver lia.
+  Qed.
+  Lemma NoDup_seq j n : NoDup (seq j n).
+  Proof. apply NoDup_ListNoDup, seq_NoDup. Qed.
+  Lemma seq_S_end_app j n : seq j (S n) = seq j n ++ [j + n].
+  Proof.
+    revert j. induction n as [|n IH]; intros j; simpl in *; f_equal; [done |].
+    by rewrite IH, Nat.add_succ_r.
+  Qed.
+
+  Lemma Forall_seq (P : nat → Prop) i n :
+    Forall P (seq i n) ↔ ∀ j, i ≤ j < i + n → P j.
+  Proof.
+    rewrite Forall_lookup. split.
+    - intros H j [??]. apply (H (j - i)), lookup_seq. lia.
+    - intros H j x [-> ?]%lookup_seq. auto with lia.
+  Qed.
+End seq.
+
+(** ** Properties of the [seqZ] function *)
+Section seqZ.
+  Implicit Types (m n : Z) (i j : nat).
+  Local Open Scope Z.
+
+  Lemma seqZ_nil m n : n ≤ 0 → seqZ m n = [].
+  Proof. by destruct n. Qed.
+  Lemma seqZ_cons m n : 0 < n → seqZ m n = m :: seqZ (Z.succ m) (Z.pred n).
+  Proof.
+    intros H. unfold seqZ. replace n with (Z.succ (Z.pred n)) at 1 by lia.
+    rewrite Z2Nat.inj_succ by lia. f_equal/=.
+    rewrite <-fmap_S_seq, <-list_fmap_compose.
+    apply map_ext; naive_solver lia.
+  Qed.
+  Lemma seqZ_length m n : length (seqZ m n) = Z.to_nat n.
+  Proof. unfold seqZ; by rewrite fmap_length, seq_length. Qed.
+  Lemma fmap_add_seqZ m m' n : Z.add m <$> seqZ m' n = seqZ (m + m') n.
+  Proof.
+    revert m'. induction n as [|n ? IH|] using (Z_succ_pred_induction 0); intros m'.
+    - by rewrite seqZ_nil.
+    - rewrite (seqZ_cons m') by lia. rewrite (seqZ_cons (m + m')) by lia.
+      f_equal/=. rewrite Z.pred_succ, IH; simpl. f_equal; lia.
+    - by rewrite !seqZ_nil by lia.
+  Qed.
+  Lemma lookup_seqZ_lt m n i : i < n → seqZ m n !! i = Some (m + i).
+  Proof.
+    revert m i. induction n as [|n ? IH|] using (Z_succ_pred_induction 0);
+      intros m i Hi; [lia| |lia].
+    rewrite seqZ_cons by lia. destruct i as [|i]; simpl.
+    - f_equal; lia.
+    - rewrite Z.pred_succ, IH by lia. f_equal; lia.
+  Qed.
+  Lemma lookup_total_seqZ_lt m n i : i < n → seqZ m n !!! i = m + i.
+  Proof. intros. by rewrite !list_lookup_total_alt, lookup_seqZ_lt. Qed.
+  Lemma lookup_seqZ_ge m n i : n ≤ i → seqZ m n !! i = None.
+  Proof.
+    revert m i.
+    induction n as [|n ? IH|] using (Z_succ_pred_induction 0); intros m i Hi; try lia.
+    - by rewrite seqZ_nil.
+    - rewrite seqZ_cons by lia.
+      destruct i as [|i]; simpl; [lia|]. by rewrite Z.pred_succ, IH by lia.
+    - by rewrite seqZ_nil by lia.
+  Qed.
+  Lemma lookup_total_seqZ_ge m n i : n ≤ i → seqZ m n !!! i = inhabitant.
+  Proof. intros. by rewrite !list_lookup_total_alt, lookup_seqZ_ge. Qed.
+  Lemma lookup_seqZ m n i m' : seqZ m n !! i = Some m' ↔ m' = m + i ∧ i < n.
+  Proof.
+    destruct (Z_le_gt_dec n i).
+    - rewrite lookup_seqZ_ge by lia. naive_solver lia.
+    - rewrite lookup_seqZ_lt by lia. naive_solver lia.
+  Qed.
+  Lemma NoDup_seqZ m n : NoDup (seqZ m n).
+  Proof. apply NoDup_fmap_2, NoDup_seq. intros ???; lia. Qed.
+
+  Lemma Forall_seqZ (P : Z → Prop) m n :
+    Forall P (seqZ m n) ↔ ∀ m', m ≤ m' < m + n → P m'.
+  Proof.
+    rewrite Forall_lookup. split.
+    - intros H j [??]. apply (H (Z.to_nat (j - m))), lookup_seqZ.
+      rewrite !Z2Nat.id by lia. lia.
+    - intros H j x [-> ?]%lookup_seqZ. auto with lia.
+  Qed.
+End seqZ.
+
+(** ** Properties of the [sum_list] and [max_list] functions *)
+Section sum_list.
+  Context {A : Type}.
+  Implicit Types x y z : A.
+  Implicit Types l k : list A.
+  Lemma sum_list_with_app (f : A → nat) l k :
+    sum_list_with f (l ++ k) = sum_list_with f l + sum_list_with f k.
+  Proof. induction l; simpl; lia. Qed.
+  Lemma sum_list_with_reverse (f : A → nat) l :
+    sum_list_with f (reverse l) = sum_list_with f l.
+  Proof.
+    induction l; simpl; rewrite ?reverse_cons, ?sum_list_with_app; simpl; lia.
+  Qed.
+  Lemma join_reshape szs l :
+    sum_list szs = length l → mjoin (reshape szs l) = l.
+  Proof.
+    revert l. induction szs as [|sz szs IH]; simpl; intros l Hl; [by destruct l|].
+    by rewrite IH, take_drop by (rewrite drop_length; lia).
+  Qed.
+  Lemma sum_list_replicate n m : sum_list (replicate m n) = m * n.
+  Proof. induction m; simpl; auto. Qed.
+  Lemma max_list_elem_of_le n ns:
+    n ∈ ns → n ≤ max_list ns.
+  Proof. induction 1; simpl; lia. Qed.
+End sum_list.
